theories/typing/type_context.v
@@ -1,9 +1,6 @@
 From iris.proofmode Require Import tactics.
 From lrust.typing Require Import type lft_contexts.
 From lrust.util Require Import types.
-Require Import Coq.Program.Equality.
-
-
 Set Default Proof Using "Type".
 
 Definition path := expr.
@@ -24,25 +21,30 @@ Notation "p ◁{ κ } ty" := (TCtx_blocked _ p κ ty%T)
 Notation pred As := (Π! As → Prop).
 Notation pred_trans As Bs := (pred Bs → pred As).
 
+Definition trans_app {As Bs Cs Ds} (tr: pred_trans As Bs) (tr': pred_trans Cs Ds)
+  : pred_trans (As ^++ Cs) (Bs ^++ Ds) :=
+  λ post bd, tr (λ a, tr' (λ c, post (a -++ c)) (psepr bd)) (psepl bd).
+
+Definition trans_tail {A Bs Cs} (tr: pred_trans Bs Cs)
+  : pred_trans (A ^:: Bs) (A ^:: Cs) :=
+  λ post '(a -:: cl), tr (λ bl, post (a -:: bl)) cl.
+
+Definition trans_upper {As Bs Cs} (tr: pred_trans As Bs)
+  : pred_trans (As ^++ Cs) (Bs ^++ Cs) :=
+  λ post ac, tr (λ b, post (b -++ psepr ac)) (psepl ac).
+
 Section type_context.
   Context `{!typeG Σ}.
 
-  Fixpoint eval_path (p : path) : option val :=
-    match p with
-    | BinOp OffsetOp e (Lit (LitInt n)) =>
-      match eval_path e with
-      | Some (#(LitLoc l)) => Some (#(l +ₗ n))
-      | _ => None
-      end
-    | e => to_val e
-    end.
+  Fixpoint eval_path (p: path) : option val := match p with
+    | BinOp OffsetOp e (Lit (LitInt n)) => match eval_path e with
+        Some (#(LitLoc l)) => Some (#(l +ₗ n)) | _ => None end
+    | e => to_val e end.
 
-  Lemma eval_path_of_val (v : val) :
-    eval_path v = Some v.
+  Lemma eval_path_of_val (v: val) : eval_path v = Some v.
   Proof. destruct v. done. simpl. rewrite (decide_left _). done. Qed.
 
-  Lemma wp_eval_path E p v :
-    eval_path p = Some v → ⊢ WP p @ E {{ v', ⌜v' = v⌝ }}.
+  Lemma wp_eval_path E p v : eval_path p = Some v → ⊢ WP p @ E {{ v', ⌜v' = v⌝ }}.
   Proof.
     revert v; induction p; intros v; try done.
     { intros [=]. by iApply wp_value. }
@@ -58,8 +60,7 @@ Section type_context.
     iIntros (v) "%". subst v. wp_op. done.
   Qed.
 
-  Lemma eval_path_closed p v :
-    eval_path p = Some v → Closed [] p.
+  Lemma eval_path_closed p v : eval_path p = Some v → Closed [] p.
   Proof.
     intros Hpv. revert v Hpv.
     induction p as [| | |[] p IH [|[]| | | | | | | | | |] _| | | | | | | |]=>//.
@@ -69,19 +70,16 @@ Section type_context.
   Qed.
 
   (** Type context element *)
-  (* TODO(xavier): Add prophecy equalizer *)
-  Definition tctx_elt_interp {A} (tid : thread_id) (x : tctx_elt A) (vπ : proph_asn → A): iProp Σ :=
-      match x with
-      | p ◁ ty =>
-        ∃v d, ⌜eval_path p = Some v⌝ ∗ ⧖d ∗ ty.(ty_own) vπ d tid [v]
-      | p ◁{κ} ty => ∃v, ⌜eval_path p = Some v⌝ ∗
-          ([†κ] ={⊤}=∗ ∃vπ' d, ▷(vπ :== vπ') ∗ ⧖d ∗ ty.(ty_own) vπ d tid [v])
-      end%I.
+  Definition tctx_elt_interp {A} (tid: thread_id) (t: tctx_elt A) (vπ: proph A)
+    : iProp Σ := match t with
+    | p ◁ ty => ∃v d, ⌜eval_path p = Some v⌝ ∗ ⧖d ∗ ty.(ty_own) vπ d tid [v]
+    | p ◁{κ} ty => ∃v, ⌜eval_path p = Some v⌝ ∗
+        ([†κ] ={⊤}=∗ ∃vπ' d, ▷(vπ :== vπ') ∗ ⧖d ∗ ty.(ty_own) vπ d tid [v]) end%I.
 
-  (* Block tctx_elt_interp from reducing with simpl when x is a constructor. *)
+  (* Block tctx_elt_interp from reducing with simpl when t is a constructor. *)
   Global Arguments tctx_elt_interp : simpl never.
 
-  Lemma tctx_hasty_val {A} tid (v : val) (ty : type A) vπ:
+  Lemma tctx_hasty_val {A} tid (v: val) (ty: _ A) vπ:
     tctx_elt_interp tid (v ◁ ty) vπ ⊣⊢ ∃d, ⧖d ∗ ty.(ty_own) vπ d tid [v].
   Proof.
     rewrite /tctx_elt_interp eval_path_of_val. iSplit.
@@ -90,12 +88,12 @@ Section type_context.
     - iDestruct 1 as (d) "[??]". eauto.
   Qed.
 
-  Lemma tctx_elt_interp_hasty_path {A} p1 p2 (ty : type A) tid vπ :
+  Lemma tctx_elt_interp_hasty_path {A} p1 p2 (ty: _ A) tid vπ :
     eval_path p1 = eval_path p2 →
     tctx_elt_interp tid (p1 ◁ ty) vπ ≡ tctx_elt_interp tid (p2 ◁ ty) vπ.
   Proof. intros Hp. rewrite /tctx_elt_interp /=. setoid_rewrite Hp. done. Qed.
 
-  Lemma tctx_hasty_val' {A} tid p (v : val) (ty : type A) vπ:
+  Lemma tctx_hasty_val' {A} tid p v (ty: _ A) vπ:
     eval_path p = Some v →
     tctx_elt_interp tid (p ◁ ty) vπ ⊣⊢ ∃ depth, ⧖depth ∗ ty.(ty_own) vπ depth tid [v].
   Proof.
@@ -105,26 +103,24 @@ Section type_context.
 
   Lemma wp_hasty {A} E tid p (ty : type A) vπ Φ :
     tctx_elt_interp tid (p ◁ ty) vπ -∗
-    (∀v d, ⌜eval_path p = Some v⌝ -∗ ⧖d -∗ ty.(ty_own) vπ d tid [v] -∗ Φ v) -∗
-    WP p @ E {{ Φ }}.
+    (∀v d, ⧖d -∗ ty.(ty_own) vπ d tid [v] -∗ Φ v) -∗ WP p @ E {{ Φ }}.
   Proof.
-    iIntros "Hty HΦ". iDestruct "Hty" as (v d ?) "(Hdepth & Hown)".
-    iApply (wp_wand with "[]"). { iApply wp_eval_path. done. }
-    iIntros (v') "%". subst v'. by iApply ("HΦ" with "[] Hdepth Hown").
+    iDestruct 1 as (???) "[#? ?]". iIntros "ToΦ".
+    iApply (wp_wand with "[]"); [by iApply wp_eval_path|].
+    iIntros (?) "->". by iApply "ToΦ".
   Qed.
 
-  Lemma closed_hasty {A} tid p (ty : type A) vπ : tctx_elt_interp tid (p ◁ ty) vπ -∗ ⌜Closed [] p⌝.
+  Lemma closed_hasty {A} tid p (ty: _ A) vπ :
+    tctx_elt_interp tid (p ◁ ty) vπ -∗ ⌜Closed [] p⌝.
   Proof. iDestruct 1 as (???) "(_ & _)". eauto using eval_path_closed. Qed.
 
-  Notation plist_pval := (plist (λ A, proph_asn → A)).
-
   (** Type context *)
-  Definition tctx_interp {As} (tid: thread_id) (T: tctx As) (vπl: plist_pval As)
+  Definition tctx_interp {As} (tid: thread_id) (T: tctx As) (vπl: plist proph As)
     : iProp Σ := [∗ hlist] t;- vπ ∈ T;- vπl, tctx_elt_interp tid t vπ.
 
   Lemma tctx_interp_singleton {A} tid (t: _ A) vπ :
     tctx_interp tid +[t] -[vπ] ⊣⊢ tctx_elt_interp tid t vπ.
-  Proof. by rewrite /tctx_interp big_sepHL2_singleton. Qed.
+  Proof. by rewrite /tctx_interp big_sepHL_1_singleton. Qed.
 
   Lemma tctx_interp_cons {A As} tid (t: _ A) (T: _ As) vπ vπl :
     tctx_interp tid (t +:: T) (vπ -:: vπl) ⊣⊢
@@ -134,23 +130,23 @@ Section type_context.
   Lemma tctx_interp_app {As Bs} tid (T: _ As) (T': _ Bs) vπl vπl' :
     tctx_interp tid (T h++ T') (vπl -++ vπl') ⊣⊢
     tctx_interp tid T vπl ∗ tctx_interp tid T' vπl'.
-  Proof. by rewrite /tctx_interp big_sepHL2_app. Qed.
+  Proof. by rewrite /tctx_interp big_sepHL_1_app. Qed.
 
   (** Copy typing contexts *)
-  Class CopyC {As: Types} (T : tctx As) vπl :=
+  Class CopyC {As} (T : tctx As) vπl :=
     copyc_persistent tid : Persistent (tctx_interp tid T vπl).
   Global Existing Instances copyc_persistent.
 
   Global Instance tctx_nil_copy : CopyC +[] -[].
   Proof. rewrite /CopyC. apply _. Qed.
 
-  Global Instance tctx_ty_copy {A As} (T : tctx As) vπl p (ty : type A) vπ:
-    CopyC T vπl → Copy ty → CopyC  ((p ◁ ty) +:: T) (vπ -:: vπl).
+  Global Instance tctx_ty_copy {A As} (T: _ As) vπl p (ty: _ A) vπ :
+    CopyC T vπl → Copy ty → CopyC (p ◁ ty +:: T) (vπ -:: vπl).
   Proof. rewrite /CopyC=> *. rewrite tctx_interp_cons. apply _. Qed.
 
   (** Send typing contexts *)
   Class SendC {As} (T: tctx As) vπl :=
-    sendc_change_tid tid1 tid2: tctx_interp tid1 T vπl ⊣⊢ tctx_interp tid2 T vπl.
+    sendc_change_tid tid1 tid2 : tctx_interp tid1 T vπl ⊣⊢ tctx_interp tid2 T vπl.
 
   Global Instance tctx_nil_send : SendC +[] -[].
   Proof. done. Qed.
@@ -179,20 +175,28 @@ Section type_context.
       by iMod (H2 with "LFT HE HL H") as "($ & $)".
   Qed. *)
 
-  Lemma tctx_incl_reflexive {As} E L (T : tctx As) : tctx_incl E L T T id.
+  Lemma tctx_incl_impl {As Bs} (T: _ As) (T': _ Bs) (tr tr': _ → _ → Prop) E L :
+    (∀post vl, tr post vl → tr' post vl) →
+    tctx_incl E L T T' tr' → tctx_incl E L T T' tr.
+  Proof.
+    move=> Imp In. iIntros (????) "#LFT E L T #Obs".
+    iMod (In with "LFT E L T []") as "$"; [|done].
+    iApply proph_obs_impl; [|done]=>/= ?. apply Imp.
+  Qed.
+
+  Lemma tctx_incl_refl {As} (T: _ As) E L : tctx_incl E L T T id.
   Proof. move=> ?? vπl ?. iIntros. iExists vπl. by iFrame. Qed.
 
-  Lemma tctx_incl_transitive E L A B C (x : tctx A) (y : tctx B) (z : tctx C) f g :
-    tctx_incl E L x y f → tctx_incl E L y z g → tctx_incl E L x z (f ∘ g).
+  Lemma tctx_incl_trans {As Bs Cs} (T1: _ As) (T2: _ Bs) (T3: _ Cs) tr tr' E L :
+    tctx_incl E L T1 T2 tr → tctx_incl E L T2 T3 tr' → tctx_incl E L T1 T3 (tr ∘ tr').
   Proof.
-    move=> H1 H2 ?? vπl ?. iIntros "#LFT #HE HL H Hp".
-    iMod (H1 with "LFT HE HL H Hp") as (?) "(HL & Hp1 & H)".
-    iMod (H2 with "LFT HE HL H Hp1") as (vπl'') "(? & Hp2 & ?)".
-    iExists vπl''. by iFrame.
+    move=> In In' >. iIntros "#LFT #E L T Obs".
+    iMod (In with "LFT E L T Obs") as (?) "(L & Obs & T)".
+    iMod (In' with "LFT E L T Obs") as (vπl'') "(?&?&?)". iExists vπl''. by iFrame.
   Qed.
 
 (*
-  Definition xprod_hsubmseteq {As Bs} {T1 : tctx As} {T2 : tctx Bs} (sub : T1 ⊆+ₕ T2) : xprod Bs → xprod As.
+  Definition xprod_hsubmseteq {As Bs} {T1 : tctx As} {T2 : tctx Bs} (sub : T1 ⊆+ₕ T2) : Π! Bs → Π! As.
     intros. dependent induction sub; simpl in *; intuition.
   Qed. *)
 
@@ -201,40 +205,38 @@ Section type_context.
     rewrite /tctx_incl. iIntros (??) "_ _ $ H". by iApply big_sepHL_submseteq.
   Qed. *)
 
-  Definition trans_app {As Bs Cs Ds} (f : pred_trans As Bs) (g : pred_trans Cs Ds)
-    : pred_trans (As ^++ Cs) (Bs ^++ Ds) :=
-    λ post bd, f (λ a, g (λ c, post (a -++ c)) (psepr bd)) (psepl bd).
-
-  Lemma tctx_incl_app {As Bs Cs Ds} E L (T1 : tctx As) (T1' : tctx Bs) f (T2: tctx Cs) (T2': tctx Ds) g:
-    tctx_incl E L T1 T1' f → tctx_incl E L T2 T2' g →
-    tctx_incl E L (T1 h++ T2) (T1' h++ T2') (trans_app f g).
+  Lemma tctx_incl_app {As Bs Cs Ds}
+    (T1: _ As) (T1': _ Bs) (T2: _ Cs) (T2': _ Ds) tr tr' E L :
+    tctx_incl E L T1 T1' tr → tctx_incl E L T2 T2' tr' →
+    tctx_incl E L (T1 h++ T2) (T1' h++ T2') (trans_app tr tr').
   Proof.
     move=> Hincl1 Hincl2 ?? vπl ?. move: (papp_ex vπl)=> [?[?->]].
     rewrite /tctx_incl tctx_interp_app.
     iIntros "#LFT #HE HL [H1 H2] HP".
     iMod (Hincl1 with "LFT HE HL H1 [HP]")  as (wπl) "(HL & Hp1 & ?)".
-    { iApply proph_obs_weaken; [|done]=> ?.
+    { iApply proph_obs_impl; [|done]=> ?.
       rewrite /trans_app papply_app papp_sepl papp_sepr. exact id. }
     iMod (Hincl2 with "LFT HE HL H2 [Hp1]") as (wπl') "(HL & Hp2 & ?)".
-    { iApply proph_obs_weaken; [|done]=> ?. exact id. }
+    { iApply proph_obs_impl; [|done]=> ?. exact id. }
     iExists (wπl -++ wπl'). rewrite tctx_interp_app. iFrame.
-    iApply proph_obs_weaken; [|done]=>/= ?. rewrite papply_app. exact id.
+    iApply proph_obs_impl; [|done]=>/= ?. rewrite papply_app. exact id.
   Qed.
 
   (* Lemma tctx_incl_frame_l {E L As Bs Cs} (T :tctx As) (T1 : tctx Bs) (T2 : tctx Cs) f:
     tctx_incl E L T1 T2 f → tctx_incl E L (T +++ T1) (T +++ T2) (xprod_bimap id f).
-  Proof. apply tctx_incl_app, tctx_incl_reflexive. Qed.
+  Proof. apply tctx_incl_app, tctx_incl_refl. Qed.
 
   Lemma tctx_incl_frame_r {E L As Bs Cs} (T : tctx As) (T1 : tctx Bs) (T2 : tctx Cs) f :
     tctx_incl E L T1 T2 f → tctx_incl E L (T1+++T) (T2+++T) (xprod_bimap f id).
-  Proof.  intros. by apply tctx_incl_app, tctx_incl_reflexive. Qed.
+  Proof.  intros. by apply tctx_incl_app, tctx_incl_refl. Qed.
   *)
 
-  Lemma tcx_incl_cons {A As Bs} E L (x : tctx_elt A) (T1 : tctx As) (T2 : tctx Bs) f :
-    tctx_incl E L T1 T2 f →
-    tctx_incl E L (x +:: T1) (x +:: T2) (trans_app (id: pred ^[A] → _) f).
+  Lemma tctx_incl_tail {A As Bs} E L (t: _ A) (T1: _ As) (T2: _ Bs) tr :
+    tctx_incl E L T1 T2 tr → tctx_incl E L (t +:: T1) (t +:: T2) (trans_tail tr).
   Proof.
-    apply (tctx_incl_app E L +[_] +[_]), tctx_incl_reflexive.
+    move=> ?. eapply tctx_incl_impl; last first.
+    { apply (tctx_incl_app +[_] +[_]); [apply tctx_incl_refl|done]. }
+    move=> ?[??]. exact id.
   Qed.
 
   (*
@@ -260,10 +262,11 @@ Section type_context.
 
   (* Extracting from a type context. *)
 
-  Definition tctx_extract_hasty {As Bs A} E L p (ty : type A) (T : tctx As) (T' : tctx Bs) f : Prop :=
-    tctx_incl E L T ((p ◁ ty) +:: T') f.
+  Definition tctx_extract_hasty {As Bs A} E L p (ty: type A)
+    (T: tctx As) (T': tctx Bs) (tr: pred_trans As (A ^:: Bs)) : Prop :=
+    tctx_incl E L T (p ◁ ty +:: T') tr.
 
-  Definition xprod_extract {As A B Bs} (f : xprod As → xprod (B ^:: Bs)) : xprod (A ^:: As) → xprod (B ^:: A ^:: Bs) :=
+  Definition xprod_extract {As A B Bs} (f : Π! As → Π! (B ^:: Bs)) : Π! (A ^:: As) → Π! (B ^:: A ^:: Bs) :=
     λ '(a -:: ass), let '(b -:: bss) := f ass in b -:: a -:: bss.
 
   (* Lemma tctx_extract_hasty_further {As Bs A B} E L p (ty : type B)  (T : tctx As) (T' : tctx Bs) f (x : tctx_elt A) :
@@ -272,7 +275,7 @@ Section type_context.
   Proof.
     rewrite /tctx_extract_hasty.
     intros.
-    eapply tctx_incl_transitive;
+    eapply tctx_incl_trans;
       [eapply tcx_incl_cons, H| apply contains_tctx_incl].
 
     Unshelve.
@@ -284,7 +287,7 @@ Section type_context.
     tctx_extract_hasty E L p1 ty' (f ∘ ) ((p2 ◁ ty)+::T) ((p2 ◁ ty [{ }])+::T) (λ p, (f p.1, p)).
   Proof.
     intros -> ??. apply (tctx_incl_frame_r _ +[_] +[_;_] (λ p, (f p.1, p))).
-    eapply tctx_incl_transitive; first by apply copy_tctx_incl, _.
+    eapply tctx_incl_trans; first by apply copy_tctx_incl, _.
     by apply (tctx_incl_frame_r _ +[_] +[_]), (subtype_tctx_incl _ _ _ _ f).
   Qed.
 
@@ -307,7 +310,7 @@ Section type_context.
   Proof.
     rewrite /tctx_extract_blocked.
     intros.
-    eapply tctx_incl_transitive;
+    eapply tctx_incl_trans;
       [eapply tcx_incl_cons, H| apply contains_tctx_incl].
 
     Unshelve.
@@ -316,32 +319,27 @@ Section type_context.
 
   (* Lemma tctx_extract_blocked_here {A As} E L p κ (ty : type A)  (T : tctx As) f:
     tctx_extract_blocked E L p κ ty  ((p ◁{κ} ty)+::T) T f.
-  Proof. intros. apply (tctx_incl_frame_r _ +[_] +[_] id), tctx_incl_reflexive. Qed. *)
+  Proof. intros. apply (tctx_incl_frame_r _ +[_] +[_] id), tctx_incl_refl. Qed. *)
 
-  Definition tctx_extract_ctx {As Bs Cs} E L (T : tctx As) (T1 : tctx Bs) (T2 : tctx Cs) f : Prop :=
-    tctx_incl E L T1 (T h++T2) f.
+  Definition tctx_extract_ctx {As Bs Cs} E L (T: tctx As)
+    (T1: tctx Bs) (T2: tctx Cs) (tr: pred_trans Bs (As ^++ Cs)) : Prop :=
+    tctx_incl E L T1 (T h++ T2) tr.
 
-  Lemma tctx_extract_ctx_nil {As} E L (T : tctx As):
-    tctx_extract_ctx E L +[] T T id.
-  Proof. apply tctx_incl_reflexive. Qed.
+  Lemma tctx_extract_ctx_nil {As} (T: _ As) E L : tctx_extract_ctx E L +[] T T id.
+  Proof. apply tctx_incl_refl. Qed.
 
-  Definition tctx_extract_ctx_hasty_trans {A As Bs Cs Ds}
-    (f : pred_trans Bs (A ^:: Cs)) (g : pred_trans Cs (As ^++ Ds))
-    : pred_trans Bs ((A ^:: As) ^++ Ds) :=
-    λ post b, f (λ '(a -:: c),  g (λ ad, post (a -:: ad)) c) b.
+  Lemma tctx_extract_ctx_hasty {A As Bs Cs Ds}
+    (ty: _ A) (T: _ As) (T1: _ Bs) (T2: _ Cs) (T3: _ Ds) p tr tr' E L :
+    tctx_extract_hasty E L p ty T1 T2 tr → tctx_extract_ctx E L T T2 T3 tr' →
+    tctx_extract_ctx E L (p ◁ ty +:: T) T1 T3 (tr ∘ trans_tail tr').
+  Proof. move=> ??. eapply tctx_incl_trans; by [|apply tctx_incl_tail]. Qed.
 
-  Lemma tctx_extract_ctx_hasty {A As Bs Cs Ds} E L (T : tctx As) (T1 : tctx Bs) (T2 : tctx Cs) (T3 : tctx Ds) p (ty : type A) f g:
-    tctx_extract_hasty E L p ty T1 T2 f → tctx_extract_ctx E L T T2 T3 g →
-    tctx_extract_ctx E L ((p ◁ ty)+::T) T1 T3 (f ∘ trans_app (id: pred ^[A] → _) g).
-  Proof. unfold tctx_extract_ctx, tctx_extract_hasty => ??.
-    eapply tctx_incl_transitive; [eassumption |  by eapply tcx_incl_cons].
-  Qed.
   (*
   Lemma tctx_extract_ctx_blocked {A As Bs Cs Ds} E L (T : tctx As) (T1 : tctx Bs) (T2 : tctx Cs) (T3 : tctx Ds) p κ (ty : type A) :
     tctx_extract_blocked E L p κ ty  T1 T2 → tctx_extract_ctx E L T T2 T3 →
     tctx_extract_ctx E L ((p ◁{κ} ty)+::T) T1 T3.
   Proof. unfold tctx_extract_ctx, tctx_extract_blocked => ?? //.
-    eapply tctx_incl_transitive, tcx_incl_cons; eassumption.
+    eapply tctx_incl_trans, tcx_incl_cons; eassumption.
   Qed.
 
   Lemma tctx_extract_ctx_incl {As Bs Cs} E L (T : tctx As) (T' : tctx Bs) (T0 : tctx Cs):
@@ -349,7 +347,7 @@ Section type_context.
     tctx_incl E L T T'.
   Proof.
     unfold tctx_extract_ctx=> ?.
-    eapply tctx_incl_transitive; first eassumption.
+    eapply tctx_incl_trans; first eassumption.
     apply contains_tctx_incl, hsubmseteq_inserts_r, hpermutation_hsubmseteq, hpermutation_refl.
   Qed. *)
 
