theories/typing/bool.v
@@ -19,16 +19,20 @@ Section bool.
 
   Lemma type_bool_instr b : typed_val #b bool_ty (λ post _, post -[b]).
   Proof.
-    iIntros (E L tid post ?) "_ _ _ $ $ _ ?". iMod persistent_time_receipt_0 as "#H0".
-    iApply wp_value. iExists -[const b]. iFrame. rewrite tctx_interp_singleton tctx_hasty_val' //.
-    iExists 0%nat. iFrame "H0". eauto.
+    iIntros (?????) "_ _ _ $$ _ ?". iMod persistent_time_receipt_0 as "#H0".
+    iApply wp_value. iExists -[const b]. iFrame.
+    rewrite tctx_interp_singleton tctx_hasty_val' //.
+    iExists 0%nat. iFrame "H0". by iExists b.
   Qed.
 
   Lemma type_bool {As} b E L C (T: _ As) x e pre:
     Closed (x :b: []) e →
-    (∀(v: val), typed_body E L C (v ◁ bool_ty +:: T) (subst' x v e) pre) -∗
+    (∀v: val, typed_body E L C (v ◁ bool_ty +:: T) (subst' x v e) pre) -∗
     typed_body E L C T (let: x := #b in e) (λ p, pre (b -:: p)).
-  Proof. iIntros. iApply type_let; by [apply type_bool_instr|solve_typing| |]. Qed.
+  Proof.
+    iIntros. iApply typed_body_impl; last first.
+    { iApply type_let; by [apply type_bool_instr|solve_typing| |]. } done.
+  Qed.
 
   Lemma type_if {As} E L C (T : tctx As) e1 e2 p pre1 pre2:
     typed_body E L C T e1 pre1 -∗ typed_body E L C T e2 pre2 -∗
@@ -37,7 +41,7 @@ Section bool.
   Proof.
     iIntros "He1 He2". iIntros (tid [bπ vπl]). rewrite tctx_interp_cons.
     iIntros "#LFT #TIME #HE Htl HL HC [Hp HT] Hv". wp_bind p.
-    iApply (wp_hasty with "Hp"). iIntros (?? _) "_".
+    iApply (wp_hasty with "Hp"). iIntros (??) "_".
     iDestruct 1 as (b->) "%Eq". move: Eq=> [=->]. wp_case. case b.
     - by iApply ("He1" with "LFT TIME HE Htl HL HC HT").
     - by iApply ("He2" with "LFT TIME HE Htl HL HC HT").
