theories/typing/uniq_cmra.v
@@ -8,14 +8,14 @@ Implicit Type (Ap: ptType) (q: Qp).
 
 (** * Camera for Unique Borrowing *)
 
-Local Definition uniq_itemR Ap := frac_agreeR (leibnizO ((proph_asn → Ap) * nat)).
+Local Definition uniq_itemR Ap := frac_agreeR (leibnizO (proph Ap * nat)).
 Local Definition uniq_gmapUR Ap := gmapUR positive (uniq_itemR Ap).
 Local Definition uniq_smryUR := discrete_funUR uniq_gmapUR.
 Definition uniqUR := authUR uniq_smryUR.
 
 Implicit Type S: uniq_smryUR.
 
-Local Definition item {Ap} q (vπd: (proph_asn → Ap) * nat) : uniq_itemR Ap :=
+Local Definition item {Ap} q (vπd: proph Ap * nat) : uniq_itemR Ap :=
   @to_frac_agree (leibnizO _) q vπd.
 Local Definition line ξ q vπd : uniq_smryUR :=
   .{[ξ.(pv_ty) := {[ξ.(pv_id) := item q vπd]}]}.
@@ -103,7 +103,7 @@ Proof.
   iMod (inv_alloc _ _ uniq_inv with "[Auth]") as "?"; by [iExists ε|].
 Qed.
 
-Definition pval_to_pt {A} (vπ: proph_asn → A) := PtType A (vπ inhabitant).
+Definition pval_to_pt {A} (vπ: proph A) := PtType A (vπ inhabitant).
 
 Lemma uniq_intro {A} E (vπ: _ → A) d :
   ↑prophN ∪ ↑uniqN ⊆ E → proph_ctx -∗ uniq_ctx ={E}=∗
